steel/Zeta.Steel.Util.fst
@@ -2,6 +2,8 @@ module Zeta.Steel.Util
 open Steel.ST.Util
 module A = Steel.ST.Array
 module U32 = FStar.UInt32
+module U64 = FStar.UInt64
+module Cast = FStar.Int.Cast
 let coerce_eq (#a:Type) (#b:Type) (_:squash (a == b)) (x:a) : b = x
 
 let full = Steel.FractionalPermission.full_perm
@@ -45,3 +47,51 @@ val release (#v:vprop) (c:cancellable_lock v)
 assume
 val cancel (#v:vprop) (c:cancellable_lock v)
   : STT unit (can_release c) (fun _ -> emp)
+
+
+let check_overflow_add32 (x y:U32.t)
+  : Pure (option U32.t)
+    (requires True)
+    (ensures fun res ->
+        if FStar.UInt.fits (U32.v x + U32.v y) 32
+        then Some? res /\
+             Some?.v res == U32.add x y
+        else None? res)
+ = let open U64 in
+   let res = U64.(Cast.uint32_to_uint64 x +^
+                  Cast.uint32_to_uint64 y)
+   in
+   if res >^ 0xffffffffuL
+   then None
+   else (assert (U64.v res  == U32.v x + U32.v y);
+         assert (U64.v res <= pow2 32);
+         let res = Cast.uint64_to_uint32 res in
+         assert (U32.v res  == U32.v x + U32.v y);
+         Some res)
+
+
+let check_overflow_add (x y:U64.t)
+  : res:option U64.t {
+        if FStar.UInt.fits (U64.v x + U64.v y) 64
+        then Some? res /\
+             Some?.v res == U64.add x y
+        else None? res
+    }
+ = let open U64 in
+   let res = U64.add_mod x y in
+   if res <^ x then None
+   else if res -^ x = y then Some res
+   else None
+
+
+let st_check_overflow_add32 (x y:U32.t)
+  : ST (option U32.t)
+       emp
+       (fun _ -> emp)
+       (requires True)
+       (ensures fun res ->
+         if FStar.UInt.fits (U32.v x + U32.v y) 32
+         then Some? res /\
+              Some?.v res == U32.add x y
+         else None? res)
+  = let r = check_overflow_add32 x y in return r
