steel/Zeta.Steel.VerifierTypes.fst
@@ -65,6 +65,10 @@ type thread_state_t = {
 
 let thread_id t = t.thread_id
 
+
+let tsm_entries_invariant (tsm:M.thread_state_model) =
+    tsm == M.verify_model (M.init_thread_state_model tsm.thread_id) tsm.processed_entries
+
 [@@__reduce__]
 let thread_state_inv (t:thread_state_t)
                      ([@@@smt_fallback] tsm:M.thread_state_model)
@@ -77,9 +81,8 @@ let thread_state_inv (t:thread_state_t)
     G.pts_to t.processed_entries full tsm.processed_entries `star`
     G.pts_to t.app_results full tsm.app_results `star`
     exists_ (A.pts_to t.serialization_buffer) `star`
-    pure (tsm == M.verify_model
-                   (M.init_thread_state_model t.thread_id)
-                   tsm.processed_entries)
+    pure (tsm_entries_invariant tsm /\
+          t.thread_id == tsm.thread_id)
 
 let elim_thread_state_inv (#o:_) (#tsm:M.thread_state_model) (t:thread_state_t)
   : STGhost unit o
